SSA/Projects/InstCombine/AliveAutoGenerated.lean
@@ -4,7 +4,7 @@ Released under Apache 2.0 license as described in the file LICENSE.
 
 import SSA.Projects.InstCombine.LLVM.PrettyEDSL
 import SSA.Projects.InstCombine.AliveStatements_sorry
-import SSA.Projects.InstCombine.Refinement
+import SSA.Projects.InstCombine.LLVM.Refinement
 import SSA.Projects.InstCombine.Tactic
 
 open MLIR AST
