SSA/Projects/InstCombine/LLVM/Refinement.lean
@@ -1,0 +1,23 @@
+/-
+Released under Apache 2.0 license as described in the file LICENSE.
+-/
+import SSA.Core.Framework
+import SSA.Core.Util.Poison
+import SSA.Projects.InstCombine.Base
+
+/-!
+## Refinement of LLVM values
+-/
+
+namespace InstCombine
+open LLVM (IntW)
+
+local instance : Refinement (BitVec w) := .ofEq
+
+instance : DialectHRefinement LLVM LLVM where
+  IsTypeCompatible := Eq
+  IsRefinedBy := @fun
+  | .bitvec w, _, Eq.refl _ => fun (x y : PoisonOr _) => x ⊑ y
+
+instance : LawfulDialectRefinement LLVM where
+  isTypeCompatible_rfl _ := rfl
