SSA/Projects/InstCombine/Tactic.lean
@@ -3,7 +3,7 @@ Released under Apache 2.0 license as described in the file LICENSE.
 -/
 import SSA.Projects.InstCombine.LLVM.EDSL
 import SSA.Projects.InstCombine.LLVM.SimpSet
-import SSA.Projects.InstCombine.Refinement
+import SSA.Projects.InstCombine.LLVM.Refinement
 import SSA.Projects.InstCombine.ForStd
 import SSA.Core.ErasedContext
 import SSA.Core.Tactic
